lib/steel/pulse/Pulse.Syntax.Naming.fsti
@@ -530,6 +530,15 @@ let close_term t v = close_term' t v 0
 let close_st_term t v = close_st_term' t v 0
 let close_comp t v = close_comp' t v 0
 
+let close_st_term_n t vs =
+  let rec aux (i:nat) (vs:list var) (t:st_term) : Tot st_term (decreases vs) =
+    match vs with
+    | [] -> t
+    | v::vs ->
+      aux (i+1) vs (close_st_term' t v i)
+  in
+  aux 0 (List.rev vs) t
+
 val close_open_inverse' (t:term) 
                         (x:var { ~(x `Set.mem` freevars t) } )
                         (i:index)
